proof/agp32_ID_CorrectScript.sml
@@ -1,4 +1,4 @@
-open hardwarePreamble translatorTheory translatorLib arithmeticTheory dep_rewrite blastLib bitstringSyntax fcpSyntax listSyntax wordsSyntax agp32StateTheory agp32EnvironmentTheory agp32ProcessorTheory ag32Theory ag32ExtraTheory ag32UtilitiesTheory agp32RelationTheory agp32UpdateTheory agp32InternalTheory agp32StepLib;
+open hardwarePreamble translatorTheory translatorLib arithmeticTheory dep_rewrite blastLib bitstringSyntax fcpSyntax listSyntax wordsSyntax agp32StateTheory agp32EnvironmentTheory agp32ProcessorTheory ag32Theory ag32ExtraTheory ag32UtilitiesTheory agp32RelationTheory agp32UpdateTheory agp32InternalTheory;
 
 (* correctness of ID stage items with respect to the ISA *)
 val _ = new_theory "agp32_ID_Correct";
@@ -84,7 +84,7 @@ Proof
     by fs [Abbr `s`,Abbr `s'`,Abbr `s''`,agp32_ID_addr_updated_by_ID_data_update] >>
   fs [ID_data_update_def] >>
   `s''.ID.ID_instr = (agp32 fext fbits (SUC t)).ID.ID_instr`
-    by fs [Abbr `s`,Abbr `s'`,Abbr `s''`,agp32_same_ID_instr_after_ID_pipeline] >> fs []
+    by fs [Abbr `s`,Abbr `s'`,Abbr `s''`,agp32_same_ID_instr_after_ID_imm_update] >> fs []
 QED
 
 
@@ -117,7 +117,62 @@ Proof
     by fs [Abbr `s`,Abbr `s'`,Abbr `s''`,agp32_ID_flag_updated_by_ID_data_update] >>
   fs [ID_data_update_def] >>
   `s''.ID.ID_instr = (agp32 fext fbits (SUC t)).ID.ID_instr`
-    by fs [Abbr `s`,Abbr `s'`,Abbr `s''`,agp32_same_ID_instr_after_ID_pipeline] >> fs []
+    by fs [Abbr `s`,Abbr `s'`,Abbr `s''`,agp32_same_ID_instr_after_ID_imm_update] >> fs []
+QED
+
+
+(** immA/B/W **)
+Theorem agp32_Rel_ag32_ID_imm_data_correct:
+  !fext fbits a t I.
+    is_sch_decode I (agp32 fext fbits) ==>
+    Rel I (fext t) (agp32 fext fbits (t-1)) (agp32 fext fbits t) a t ==>
+    enable_stg 2 (agp32 fext fbits t) ==>
+    I (2,SUC t) <> NONE ==>
+    ((agp32 fext fbits (SUC t)).ID.ID_immA = immA (FUNPOW Next (THE (I (2,SUC t)) − 1) a)) /\
+    ((agp32 fext fbits (SUC t)).ID.ID_immB = immB (FUNPOW Next (THE (I (2,SUC t)) − 1) a)) /\
+    ((agp32 fext fbits (SUC t)).ID.ID_immW = immW (FUNPOW Next (THE (I (2,SUC t)) − 1) a))
+Proof
+  rpt gen_tac >> rpt disch_tac >>
+  simp [immA_def,immB_def,immW_def] >>
+  `(agp32 fext fbits (SUC t)).ID.ID_instr = instr (FUNPOW Next (THE (I' (2,SUC t)) − 1) a)`
+    by fs [agp32_Rel_ag32_ID_instr_correct] >>
+  Q.ABBREV_TAC `s = agp32 fext fbits t` >>
+  Q.ABBREV_TAC `s' = procs [agp32_next_state; WB_pipeline; MEM_pipeline; EX_pipeline;
+                            REG_write; ID_pipeline; IF_PC_update; Acc_compute] (fext t) s s` >>
+  Q.ABBREV_TAC `s'' = procs [ForwardA; ForwardB; ForwardW; IF_instr_update; ID_opc_func_update;
+                             ID_imm_update] (fext (SUC t)) s' s'` >>                          
+  `?s0. (agp32 fext fbits (SUC t)).ID.ID_immA = (ID_data_update (fext (SUC t)) s0 s'').ID.ID_immA /\
+  (agp32 fext fbits (SUC t)).ID.ID_immB = (ID_data_update (fext (SUC t)) s0 s'').ID.ID_immB /\
+  (agp32 fext fbits (SUC t)).ID.ID_immW = (ID_data_update (fext (SUC t)) s0 s'').ID.ID_immW`
+    by fs [Abbr `s`,Abbr `s'`,Abbr `s''`,agp32_ID_imm_data_updated_by_ID_data_update] >>
+  fs [ID_data_update_def] >>
+  `s''.ID.ID_instr = (agp32 fext fbits (SUC t)).ID.ID_instr`
+    by fs [Abbr `s`,Abbr `s'`,Abbr `s''`,agp32_same_ID_instr_after_ID_imm_update] >> fs []
+QED
+
+
+(** imm for LoadConstant and LoadUpperConstant **)
+Theorem agp32_Rel_ag32_ID_imm_correct:
+  !fext fbits a t I.
+    is_sch_decode I (agp32 fext fbits) ==>
+    Rel I (fext t) (agp32 fext fbits (t-1)) (agp32 fext fbits t) a t ==>
+    enable_stg 2 (agp32 fext fbits t) ==>
+    I (2,SUC t) <> NONE ==>
+    (agp32 fext fbits (SUC t)).ID.ID_imm = imm (FUNPOW Next (THE (I (2,SUC t)) − 1) a)
+Proof
+  rw [] >>
+  `(agp32 fext fbits (SUC t)).ID.ID_instr = instr (FUNPOW Next (THE (I' (2,SUC t)) − 1) a)`
+    by fs [agp32_Rel_ag32_ID_instr_correct] >>
+  Q.ABBREV_TAC `s = agp32 fext fbits t` >>
+  Q.ABBREV_TAC `s' = procs [agp32_next_state; WB_pipeline; MEM_pipeline; EX_pipeline;
+                            REG_write; ID_pipeline; IF_PC_update; Acc_compute] (fext t) s s` >>
+  Q.ABBREV_TAC `s'' = procs [ForwardA; ForwardB; ForwardW; IF_instr_update; ID_opc_func_update]
+                            (fext (SUC t)) s' s'` >>
+  `(agp32 fext fbits (SUC t)).ID.ID_imm = (ID_imm_update (fext (SUC t)) s' s'').ID.ID_imm`
+    by fs [Abbr `s`,Abbr `s'`,Abbr `s''`,agp32_ID_imm_updated_by_ID_imm_update] >>
+  `s''.ID.ID_instr = (agp32 fext fbits (SUC t)).ID.ID_instr`
+    by fs [Abbr `s`,Abbr `s'`,Abbr `s''`,agp32_same_ID_instr_after_ID_opc_func_update] >>
+   fs [ID_imm_update_def,imm_def] >> rw []
 QED
 
 
@@ -130,11 +185,10 @@ Theorem agp32_Rel_ag32_ID_Rel_correct:
     I (2,SUC t) <> NONE ==>
     ID_Rel (fext (SUC t)) (agp32 fext fbits (SUC t)) a (THE (I (2,SUC t)))
 Proof
-  rw [ID_Rel_def] >-
-   fs [agp32_Rel_ag32_ID_PC_correct] >-
-   fs [agp32_Rel_ag32_ID_instr_correct] >>
-  fs [agp32_Rel_ag32_ID_addr_correct] >>
-  fs [agp32_Rel_ag32_ID_flag_correct] >>
+  rw [ID_Rel_def] >>
+  fs [agp32_Rel_ag32_ID_PC_correct,agp32_Rel_ag32_ID_instr_correct,agp32_Rel_ag32_ID_addr_correct,
+      agp32_Rel_ag32_ID_flag_correct,agp32_Rel_ag32_ID_imm_data_correct,
+      agp32_Rel_ag32_ID_imm_correct] >>
   cheat
 QED
 
